Control.v
@@ -6,5 +6,5 @@ Require Export Control.CommutativeApplicative.
 Require Export Control.Foldable.
 Require Export Control.Functor.
 Require Export Control.Monad.
-Require Export Control.Monad.MonadPlus.
+(*Require Export Control.Monad.MonadPlus.*)
 Require Export Control.Monad.Trans.
