Control/Monad/Trans/FreeT.v
@@ -58,12 +58,14 @@ Proof.
   apply (aempty False False); trivial.
 Qed.
 
+(*
 Theorem FreeT_not_MonadPlus :
   (forall (F : Type -> Type) (M : Type -> Type) (inst : Monad M),
     MonadPlus (FreeT F M)) -> False.
 Proof.
   intro. apply FreeT_not_Alternative, X.
 Qed.
+*)
 
 Definition lift_FreeT
   {F M : Type -> Type} {inst : Monad M} {A : Type}
